ott_coq/ext_nat.v
@@ -1,4 +1,5 @@
 Require Import Ott.ott_list_core.
+Require Import Arith.
 
 Inductive ext_nat : Type :=
     | Fin : nat -> ext_nat
@@ -13,3 +14,15 @@ Definition ext_plus (m n : ext_nat) : ext_nat :=
 
 Definition ext_plus' (l : list ext_nat) : ext_nat :=
   List.fold_left ext_plus l (Fin 0).
+
+Theorem ext_eq_dec : forall m n : ext_nat, {m = n} + {m <> n}.
+Proof.
+  decide equality.
+  apply eq_nat_dec.
+Defined.
+
+Definition ext_eqb (m n : ext_nat) : bool :=
+  match ext_eq_dec m n with
+  | left _ => true
+  | right _ => false
+  end.
